vale/code/arch/x64/interop/GCMencryptOpt_stdcalls.fst
@@ -4,6 +4,7 @@ open Vale.Stdcalls.GCMencryptOpt
 open Vale.AsLowStar.MemoryHelpers
 open X64.MemoryAdapters
 module V = X64.Vale.Decls
+open Simplify_Sha
 open Gcm_simplify
 open GCM_helpers
 open FStar.Calc
@@ -688,104 +689,6 @@ let gcm128_encrypt_opt_alloca key plain_b plain_len auth_b auth_bytes iv_b
   let h_f = get() in
   gcm_simplify2 tag_b h_f
 
-(*
-inline_for_extraction
-val gcm128_encrypt_opt_stdcall':
-  key:Ghost.erased (Seq.seq nat32) ->
-  plain_b:uint8_p ->
-  plain_len:uint64 ->
-  auth_b:uint8_p ->
-  auth_len:uint64 ->
-  iv_b:uint8_p ->
-  out_b:uint8_p ->
-  tag_b:uint8_p ->
-  keys_b:uint8_p ->
-  hkeys_b:uint8_p ->
-
-  Stack unit
-    (requires fun h0 ->
-      B.disjoint tag_b out_b /\ B.disjoint tag_b hkeys_b /\
-      B.disjoint tag_b plain_b /\ B.disjoint tag_b auth_b /\
-      disjoint_or_eq tag_b iv_b /\ disjoint_or_eq tag_b keys_b /\
-
-      B.disjoint iv_b keys_b /\ B.disjoint iv_b out_b /\
-      B.disjoint iv_b plain_b /\ B.disjoint iv_b hkeys_b /\
-      B.disjoint iv_b auth_b /\
-
-      B.disjoint out_b keys_b /\ B.disjoint out_b hkeys_b /\
-      B.disjoint out_b auth_b /\ disjoint_or_eq out_b plain_b /\
-      
-      B.disjoint plain_b keys_b /\ B.disjoint plain_b hkeys_b /\
-      B.disjoint plain_b auth_b /\
-
-      disjoint_or_eq keys_b hkeys_b /\ 
-      B.disjoint keys_b auth_b /\ B.disjoint hkeys_b auth_b /\
-
-      B.live h0 auth_b /\ B.live h0 keys_b /\
-      B.live h0 iv_b /\ B.live h0 hkeys_b /\
-      B.live h0 out_b /\ B.live h0 plain_b /\
-      B.live h0 tag_b /\
-
-      B.length auth_b = UInt64.v auth_len /\
-      B.length iv_b = 16 /\
-      B.length plain_b = UInt64.v plain_len /\
-      B.length out_b = B.length plain_b /\
-      B.length hkeys_b = 160 /\
-      B.length tag_b == 16 /\
-      B.length keys_b = 176 /\
-
-      4096 * (UInt64.v plain_len) < pow2_32 /\
-      4096 * (UInt64.v auth_len) < pow2_32 /\
-
-      aesni_enabled /\ pclmulqdq_enabled /\
-      is_aes_key_LE AES_128 (Ghost.reveal key) /\
-      (let db = get_downview keys_b in
-      length_aux keys_b;
-      let ub = UV.mk_buffer db Views.up_view128 in
-      Seq.equal (UV.as_seq h0 ub) (key_to_round_keys_LE AES_128 (Ghost.reveal key)))
-    )
-    (ensures fun h0 _ h1 ->
-      B.modifies (B.loc_union (B.loc_buffer tag_b)
-                 (B.loc_union (B.loc_buffer iv_b)
-                 (B.loc_buffer out_b))) h0 h1 /\
-
-      (length_aux4 iv_b;
-       DV.length_eq (get_downview iv_b);
-       let iv_LE = low_buffer_read TUInt8 TUInt128 h0 iv_b 0 in
-       let iv_BE = reverse_bytes_quad32 iv_LE in
-       let ctr_BE_1 = Mkfour 1 iv_BE.lo1 iv_BE.hi2 iv_BE.hi3 in
-       let ctr_BE_2 = Mkfour 2 iv_BE.lo1 iv_BE.hi2 iv_BE.hi3 in
-
-      let plain_in = le_bytes_to_seq_quad32 (pad_to_128_bits (seq_uint8_to_seq_nat8 (B.as_seq h0 plain_b))) in
-      let cipher_out = le_bytes_to_seq_quad32 (pad_to_128_bits (seq_uint8_to_seq_nat8 (B.as_seq h1 out_b))) in
-
-       DV.length_eq (get_downview hkeys_b);
-       let h = reverse_bytes_quad32 (low_buffer_read TUInt8 TUInt128 h1 hkeys_b 0) in
-       let length_quad = reverse_bytes_quad32 (Mkfour (8 * UInt64.v plain_len) 0 (8 * UInt64.v auth_len) 0) in
-      let auth_pad = le_bytes_to_seq_quad32 (pad_to_128_bits (seq_uint8_to_seq_nat8 (B.as_seq h0 auth_b))) in
-      let auth_in = Seq.append auth_pad (Seq.append cipher_out (Seq.create 1 length_quad)) in
-
-      DV.length_eq (get_downview tag_b);
-      low_buffer_read TUInt8 TUInt128 h1 tag_b 0 ==
-         gctr_encrypt_block ctr_BE_1 (ghash_LE h auth_in) AES_128 (Ghost.reveal key) 0 /\
-       gctr_partial AES_128 (B.length plain_b / 16 + 1) plain_in cipher_out (Ghost.reveal key) ctr_BE_2)
-    )
-*)
-
-(*
-let length_aux6 (b:uint8_p) : Lemma
-  (requires B.length b = 16)
-  (ensures DV.length (get_downview b) / 16 = 1) =
-    let db = get_downview b in
-    DV.length_eq db  
-
-let length_aux7 (b:uint8_p) : Lemma
-  (requires B.length b = 160)
-  (ensures DV.length (get_downview b) / 16 = 10) =
-    let db = get_downview b in
-    DV.length_eq db  
-*)
-
 let lemma_identical_uv (b:uint8_p) (h0 h1:HS.mem) : Lemma
   (requires B.length b % 16 = 0 /\ Seq.equal (B.as_seq h0 b) (B.as_seq h1 b))
   (ensures (
@@ -802,9 +705,10 @@ let length_aux6 (b:uint8_p) : Lemma (B.length b = DV.length (get_downview b))
   = DV.length_eq (get_downview b)
 
 let lemma_slice_uv_extra (b:uint8_p) (b_start:uint8_p) (b_extra:uint8_p) (h:HS.mem) : Lemma
-  (requires
-    B.length b_extra = 16 /\ B.length b_start % 16 = 0 /\
-    B.length b_extra + B.length b_start >= B.length b /\
+  (requires 
+    B.length b_start = B.length b / 16 * 16 /\
+    b_start == B.gsub b 0ul (UInt32.uint_to_t (B.length b_start)) /\ 
+    B.length b_extra = 16 /\
     Seq.equal 
       (B.as_seq h b)
       (Seq.slice (Seq.append (B.as_seq h b_start) (B.as_seq h b_extra)) 0 (B.length b))
@@ -823,8 +727,68 @@ let lemma_slice_uv_extra (b:uint8_p) (b_start:uint8_p) (b_extra:uint8_p) (h:HS.m
     in let sf = slice_work_around (le_seq_quad32_to_bytes suv) (B.length b) in
     Seq.equal sf (seq_uint8_to_seq_nat8 (B.as_seq h b))
  ))
- = admit()
-
+ =
+ let b_start_d = get_downview b_start in
+ length_aux6 b_start;
+ let b_start_u = UV.mk_buffer b_start_d Views.up_view128 in
+ let b_extra_d = get_downview b_extra in
+ length_aux6 b_extra;
+ let b_extra_u = UV.mk_buffer b_extra_d Views.up_view128 in
+ let suv =
+   if B.length b > B.length b_start then
+     Seq.append (UV.as_seq h b_start_u) (UV.as_seq h b_extra_u)
+   else UV.as_seq h b_start_u
+ in let sf = slice_work_around (le_seq_quad32_to_bytes suv) (B.length b) in
+ let b_f = seq_uint8_to_seq_nat8 (B.as_seq h b) in
+ if B.length b > B.length b_start then (
+   calc (==) {
+     sf;
+     (==) { DV.length_eq b_start_d; lemma_seq_nat8_le_seq_quad32_to_bytes_uint32 b_start h;
+          le_bytes_to_seq_quad32_to_bytes (UV.as_seq h b_start_u) }
+     slice_work_around (le_seq_quad32_to_bytes (Seq.append 
+       (le_bytes_to_seq_quad32 (seq_uint8_to_seq_nat8 (B.as_seq h b_start)))
+       (UV.as_seq h b_extra_u)))
+     (B.length b);
+     (==) { DV.length_eq b_extra_d; lemma_seq_nat8_le_seq_quad32_to_bytes_uint32 b_extra h;
+       le_bytes_to_seq_quad32_to_bytes (UV.as_seq h b_extra_u) }
+     slice_work_around (le_seq_quad32_to_bytes (Seq.append 
+       (le_bytes_to_seq_quad32 (seq_uint8_to_seq_nat8 (B.as_seq h b_start)))
+       (le_bytes_to_seq_quad32 (seq_uint8_to_seq_nat8 (B.as_seq h b_extra)))))
+     (B.length b);
+     (==) { append_distributes_le_seq_quad32_to_bytes
+        (le_bytes_to_seq_quad32 (seq_uint8_to_seq_nat8 (B.as_seq h b_start)))
+        (le_bytes_to_seq_quad32 (seq_uint8_to_seq_nat8 (B.as_seq h b_extra)))
+        }
+     slice_work_around (Seq.append
+       (le_seq_quad32_to_bytes (le_bytes_to_seq_quad32 (seq_uint8_to_seq_nat8 (B.as_seq h b_start))))
+       (le_seq_quad32_to_bytes (le_bytes_to_seq_quad32 (seq_uint8_to_seq_nat8 (B.as_seq h b_extra)))))
+     (B.length b);
+     (==) { le_seq_quad32_to_bytes_to_seq_quad32 (seq_uint8_to_seq_nat8 (B.as_seq h b_start));
+            le_seq_quad32_to_bytes_to_seq_quad32 (seq_uint8_to_seq_nat8 (B.as_seq h b_extra)) }
+     slice_work_around (Seq.append
+       (seq_uint8_to_seq_nat8 (B.as_seq h b_start))
+       (seq_uint8_to_seq_nat8 (B.as_seq h b_extra)))
+     (B.length b);
+     (==) { Seq.lemma_eq_intro b_f
+       (slice_work_around (Seq.append
+         (seq_uint8_to_seq_nat8 (B.as_seq h b_start))
+         (seq_uint8_to_seq_nat8 (B.as_seq h b_extra)))
+       (B.length b))
+     }
+     b_f;
+   }
+ ) else (
+   calc (==) {
+     sf;
+     (==) { }
+     slice_work_around (le_seq_quad32_to_bytes (UV.as_seq h b_start_u)) (B.length b);
+     (==) {    DV.length_eq (get_downview b_start);
+               gcm_simplify1 b_start h (B.length b) }
+     seq_uint8_to_seq_nat8 (B.as_seq h b_start);
+     (==) { }
+     b_f;
+   }
+ )
 
 let lemma_slice_sub (b:uint8_p) (b_sub:uint8_p) (b_extra:uint8_p) (h:HS.mem) : Lemma
   (requires B.length b_extra = 16 /\ B.length b_sub = B.length b / 16 * 16 /\
